A sequence (of real numbers) is some list of real numbers, one for each $n\in\mathbb{N}$ 
- Don't have to be given by some formula, can be random
	- **Ex)** The terms could be given by calling a die
- Must be infinitely long

More precisely:
 A Sequence (of real numbers) is a function $a:\mathbb{N} \to \mathbb{R}$
 - Rather than $a(1), a(2)\dots$, we use $a_{1}, a_{2}\dots$ for each term of the sequence
 - Often write the entire sequence as $\{a_{n}\}$
	 - $\{a_{n}\}^{\infty}_{n=1}$
	 - $\{a_{n}\}_{n\in\mathbb{N}}$

Can be specified using
1) A pattern (e.g. $2,4,6,8\dots$)
2) A Formula, (e.g. $a_{n}=(-1)^{n}$)
3) A Recursive Formula, ($a_{1}=1, a_{2}=2, \text{ For }n>2, a_{n}=a_{n-1}+a_{n-2}$)
4) Or by a case
	- $a_{n}=5 \text{ if }n<10$
	- $a_{n}=10 \text{ if }10\leq n<20$
	- $a_{n}=6.8 \text{ if }n\geq 20$

# Convergence
Some sequence "Set close to a specified value" 
- i.e. Converge to Something
- $\left\{ \frac{1}{n} \right\}$ converges to 0
- $\{(-1)^{n}\}$ does not converge to something
- $\left\{ \frac{(-1)^{n}}{n} \right\}$ converges to 0
	- Note that this converge neither its $\sup$ nor $\text{inf}$

Suppose $\{a_{n}\}$ is a sequence and $L$ is some real number, We say that $\{a_{n}\}$ converges to $L$ if $\forall \text{ }\epsilon\in \mathbb{R}, \epsilon\geq 0$, there is some $K\in\mathbb{R}$ so that for any natural number $n$ with $n>K$,
$$L-\epsilon<a_{n}<L+\epsilon$$
- $\lim_{n\to \infty}{a_{n}}=L$

No matter how small $\epsilon$ is, you can find a point after which all terms in the sequence are within $\epsilon$ distance of $L$

## Example: Prove $\left\{ \frac{1}{n} \right\}$ converges to 0
Let $\epsilon>0$. Then, let's take $K=\frac{1}{\epsilon}$
- Sometimes we need to do "rough work" first

Let $n\in\mathbb{N}$ so that $n>K$, we know have to show $L-\epsilon<a_{n}<L+\epsilon$
 $\implies$ Show $-\epsilon<\frac{1}{n}<\epsilon$ for such $n$

i) $-\epsilon<\frac{1}{n}$
This is true since $\epsilon>0$, $-\epsilon<0$ and $\forall \text{ } n\in\mathbb{N}$, $n>0$ so $\frac{1}{n}>0$
- Thus, $-\epsilon<\frac{1}{n}$

ii) $\frac{1}{n}<\epsilon$
Since $K=\frac{1}{\epsilon}\implies \epsilon=\frac{1}{K}$
- $n>K,\frac{1}{n}<\frac{1}{K}=\epsilon$ 

Therefore, $-\epsilon<\frac{1}{n}<\epsilon$, $\frac{1}{n}$ converges to 0 by definition

## Example: Show $\left\{ \frac{1}{n} \right\}$ does not converge to -1
We want to show that for some $\epsilon>0$ tha definition fails

Let $\epsilon=\frac{1}{2}$. We need to find $k$ such that $\forall \text{ }n>K$, $L-\epsilon<a_{n}<L+\epsilon$
 $\implies -1.5<\frac{1}{n}<0.5$
- Since $n>0$, $a_{n}=\frac{1}{n}>0$. This is never satisfied

Thus, $\{a_{n}\}$ does not converge to -1

# Absolute Value
If $a\in\mathbb{R}$, define $|a|$
- $=a\text{ }(a\geq0)$
- $=-a\text{ }(a<0)$

## Properties
1) $|ab|=|a| |b|$
2) $|a+b|\leq|a|+|b|$

## Absolute Value form of Convergense
$\lim_{n\to \infty}{a_{n}}=L$ if and only if
$$\forall \text{ }\epsilon>0\text{ , }\exists \text{ }K\text{ S.T }\forall \text{ }n>K\text{ , }|a_{n}-L|<\epsilon$$
- We can consider $|a_{n}-L|$ be a distance between $a_{n}$ and $L$

## Example: Prove $\left\{ \frac{(-1)^{n}}{n} \right\}$ converges to 0
Let $\epsilon>0$, let's take $K=\frac{1}{\epsilon}$

Let $n>K$. We want to show $|a_{n}-L|<\epsilon$
- Here, $$|a_{n}-L|=\left|\frac{(-1)^{n}}{n}\right|=|(-1)^{n}| \left| \frac{1}{n}\right|=\frac{1}{n}<\frac{1}{K}$$
 Since $n>k$
$$=\frac{1}{\frac{1}{\epsilon}}=\epsilon$$
Meanwhile, 
$$-\epsilon<0<\frac{1}{n}\implies -\epsilon<\frac{1}{n}$$
$$\therefore-\epsilon<\frac{1}{n}<\epsilon$$
## Example: Show $\lim_{n\to \infty}{\left( 2+\frac{3}{n} \right)}=2$
Rough work first
- $|a_{n}-{L}|=|2+\frac{3}{n}-2|=\left|\frac{3}{n}\right|=\frac{3}{n}<\epsilon$
	- $\frac{3}{\epsilon}<n$
	- It looks like $K=\frac{3}{\epsilon}$ should work

Let $\epsilon>0$, set $K=\frac{3}{\epsilon}$. Let $n>K$

Consider $|a_{n}-L|=|2+\frac{3}{n}-2|=\left|\frac{3}{n}\right|=\frac{3}{n}$

$n>0,\frac{3}{n}>0$. Then, $\frac{3}{n}<\frac{3}{K}$(Since $n>K$)
- $<\frac{3}{K}=\frac{3}{\frac{3}{\epsilon}}=\epsilon$
$\therefore \forall \text{ }n>K\text{ , }|a_{n}-L|<\epsilon$

# Convergence of Complicate Sequence
To figure out more complicate sequence convergence, we need to prove "limit respect arithmetic operation"

First, we need to talk about boundness
## Bounded
Say a sequence is bounded above if its set of points is bounded above(similarly for bounded below). 
- Say sequence $\{a_{n}\}$ is **bounded** if it is bounded above and below
- $\exists \text{ }b_{1},b_{2}\in\mathbb{R}$ so that $\forall \text{ }n\in\mathbb{N}, b_{1}\leq n\leq b_{2}$

## Exercise
Show that $\{a_{n}\}$ is bounded iff there exists some $b\in\mathbb{R}$ such that $\forall \text{ }n\in\mathbb{N}$, $|a_{n}|\leq b$

## Prop 24. If $\{a_{n}\}$ is a sequence and converges to some $L\in\mathbb{R}$ then $\{a_{n}\}$ is bounded
If we let $\epsilon=1$ (any $\epsilon$ is fine)
Since the sequence converges to $L$,  there is some $K$ such that 
$$\forall \text{ }n>K, L-1<a_{n}<L+1$$
- We know that sequence is bounded after $K$, how about rest?

Since $K$ is finite, in the rest of sequence, there are only finite number $n\leq K$, so this set itself is also bounded above and below
- More specifically, has max and min

**NOTE)** This doesn't mean that bounded sequence is convergent

# Theorem 25. Sequence Arithmetic Theorem
If $\{a_{n}\}$ and $\{b_{n}\}$ are sequences and $\lim_{n\to \infty}{a_{n}}=L, \lim_{n\to \infty}{b_{n}}=M$

## 1) For any $a\in\mathbb{R}, \lim_{n\to \infty}{a}=a$
Let $\epsilon>0$, need $|a_{n}-L|<\epsilon$ $\forall \text{ }n>K$
In this case, $a_{n}=a$ and $L=a$. If we take any $K$, then for any $n>K$,
$|a_{n}-L|$
$=|a-a|$
$=|0|$
$=0<\epsilon$ $\implies$ $\{a_{n}\}$ converges to $a$

## 2) For any $c\in\mathbb{R}$, $\lim_{n\to \infty}{ca_{n}}=cL=c\lim_{n\to \infty}{a_{n}}$


## 3) $\lim_{n\to \infty}{a_{n}+b_{n}}=L+M=\lim_{n\to \infty}{a_{n}}+\lim_{n\to \infty}{b_{n}}$
Rough Work, need to set $|(a_{n}+b_{n})-(L+M)|<\epsilon$
 $\implies$ $|(a_{n}-L)+(b_{n}-M)|\leq |a_{n}-L|+|b_{n}-M|$ by triangular inequality

We need to set each term $<\frac{\epsilon}{2}$ ($|a_{n}-L|<\frac{\epsilon}{2}$ & $|b_{n}-L|<\frac{\epsilon}{2}$), then the result would be $<\epsilon$

Let $\epsilon>0$. 
Then, since $\{a_{n}\}$ conv to $L$, there is some $K_{1}$ such that $\forall \text{ }n>K_{1}$ $|a_{n}-L|<\frac{\epsilon}{2}$
And some $K_{2}$ such that $\forall \text{ }n>K_{2}$ $|b_{n}-M|<\frac{\epsilon}{2}$
- Be careful: these $K$'s might be different

Then take $K=\max(K_{1},K_{2})$ not let $n>K$

Then, $|(a_{n}+b_{n})-(L+M)|=|(a_{n}-L)+(b_{n}-M)|\leq |a_{n}-L|+|b_{n}-M|<\frac{\epsilon}{2}+\frac{\epsilon}{2}=\epsilon$

So we've satisfied the definition of convergence, so indeed $\lim_{n\to \infty}{(a_{n}+b_{n})}=L+M$

## 4) $\lim_{n\to \infty}{a_{n}b_{n}}=LM=\lim_{n\to \infty}{a_{n}}\lim_{n\to \infty}{b_{n}}$
Rough Work First
- We'll need to set $|a_{n}b_{n}-LM|$ small
- And we can get $|a_{n}-L|$ and $|b_{n}-M|$ are small

$n=|a_{n}b_{n}-a_{n}M+a_{n}M-LM|$
$\leq|a_{n}b_{n}-a_{n}M|+|a_{n}M-LM|$ by triangular ine
$=|a_{n}| |b_{n}-M|+|M| |a_{n}-L|$ abs property
- We can make $|a_{n}-L|<\frac{\epsilon}{2|M|}$
- Since $\{a_{n}\}$ converges by Lemma 24, $\exists \text{ }$some $B$ so that $\forall \text{ }n\in\mathbb{N}$, $|a_{n}|\leq B$
	- Thus, we can make $|b_{n}-M|<\frac{\epsilon}{2B}$

**Formal Proof)**
Let $\epsilon>0$
Since $\{a_{n}\}$ converges to $L$, there is some $B\in\mathbb{R}$ so that $\forall \text{ } n\in\mathbb{N}, a_{n}\leq B$

Since $\{a_{n}\}$ converges to $L$ there is some $K_{1}\in\mathbb{R}$ so that $\forall \text{ } n>K_{1}$, $|a_{n}-L|<\frac{\epsilon}{2|M|}$

Since $\{b_{n}\}$ converges to $M$, there is some $K_{2}\in\mathbb{R}$ so that $\forall \text{ }n>K_{2}, |b_{n}-M|<\frac{\epsilon}{2B}$

Let $K=\max(K_{1}, K_{2})$. Then, suppose $n>K$
$$|a_{n}b_{n}-LM|=|a_{n}b_{n}-a_{n}M+a_{n}M-LM|$$
$$\leq |a_{n}b_{n}-a_{n}M|+|a_{n}M-LM|=|a_{n}| |b_{n}-M|+|M| |a_{n}-L|$$
$$<B\cdot \frac{\epsilon}{2B}+|M|\cdot \frac{\epsilon}{2|M|}$$
$$=\frac{\epsilon}{2}+\frac{\epsilon}{2}=\epsilon$$

Therefore, we've satisfied the convergence definition.

However, we don't know that $M$ is non-zero
- Thus, we need to take the separate the case for $M=0$
- For $B$, if $B=0$, then just take $B=1$

If $M=0$
(Exercise)

## 5) If $\forall \text{ }n\in\mathbb{N} , b_{n}\neq 0$ and $M\neq 0$, then $\lim_{n\to \infty}{\frac{a_{n}}{b_{n}}}=\frac{L}{M}$
Prove $\lim_{n\to \infty}{\frac{1}{b_{n}}}=\frac{1}{M}$ first, then use 4) property 

# Theorem 26. Sequeeze Theorem for Sequence
If there are sequences $\{a_{n}\}, \{b_{n}\}, \{c_{n}\}$, with $\forall \text{ }n\in\mathbb{N}, a_{n}\leq b_{n} \leq c_{n}$ and there is a real number $L$ so that $\lim_{n\to \infty}{a_{n}}=\lim_{n\to \infty}{c_{n}}=L$.
- Then, $\lim_{n\to \infty}{b_{n}}$

## Example) $\lim_{n\to \infty}{\frac{\sin n}{n}}$
Since $-1\leq\sin n\leq 1$, $\frac{-1}{n}\leq\frac{\sin n}{n}\leq\frac{1}{n}$
Since $\lim_{n\to \infty}{\frac{-1}{n}}=\lim_{n\to \infty}{\frac{1}{n}}=0$ by the arithmetic theorem
- Then, $\lim_{n\to \infty}{\frac{\sin n}{n}}=0$ by the sequeeze theorem

## Proof)
Let $\epsilon>0$, we need $K$ so that $\forall \text{ }n>K, L-\epsilon<b_{n}<L+\epsilon$

Since $\{a_{n}\}$ converges to $L$, there is some $K_{1}$
 so that $\forall \text{ }n>K_{1}$, $L-\epsilon<a_{n}<L+\epsilon$

Since $\{c_{n}\}$ converges to $L$, there is some $K_{2}$
 so that $\forall \text{ }n>K_{2}$, $L-\epsilon<c_{n}<L+\epsilon$

Then, $b_{n}\leq c_{n}<L+\epsilon$ and $L-\epsilon<a_{n}\leq b_{n}$

Therefore, $L-\epsilon<b_{n}<L+\epsilon$ for $\forall \text{ }n>K$

# Increasing & Decreasing Sequence
A sequence is increasing if $\forall \text{ }n\in\mathbb{N}, a_{n}\leq a_{n+1}$
- Strictly increasing if $\forall \text{ }n\in\mathbb{N}, a_{n}< a_{n+1}$

A sequence is decreasing if $\forall \text{ }n\in\mathbb{N}, a_{n}\geq a_{n+1}$
- Strictly decreasing if $\forall \text{ }n\in\mathbb{N}, a_{n}> a_{n+1}$

# Theorem 27. Monotone Convergence Theorem
## If a sequence $\{a_{n}\}$ is increasing and bounded above, then it converges to $\text{sup}(\{a_{n}:n\in\mathbb{N}\})$
Since $\{a_{n}\}$ is bounded above, the set $\{a_{n}:n\in\mathbb{N}\}$ is bounded above and non-empty($a_{1}$ is in the set), so by the completeness axiom, $\text{sup}$ exists, call it $L$

Then, we want to show $\lim_{n\to \infty}{a_{n}=L}$. Let $\epsilon>0$, we need a $K$ so that $\forall \text{ }n>K$
$$L-\epsilon<a_{n}<L+\epsilon$$
Since $L$ is an upper bound, $\forall \text{ }n\in \mathbb{N}, a_{n}\leq L<L+\epsilon$

Also, Since $L$ is upper bound, $L-\epsilon$ is not an upper bound for $\{a_{n}:n\in\mathbb{N}\}$
- Therefore, there is some term in the sequence, $a_{K}$, for which $L-\epsilon<a_{K}$

But, now we claim that for any $n>K$, $L-\epsilon<a_{n}$ 
- Remember that $\{a_{n}\}$ is increasing, $a_{n}\geq a_{K}$

Therefore, 
$$L-\epsilon<a_{K}\leq  a_{n}<L+\epsilon$$

For any $n>K$, $L-\epsilon<a_{n}<L+\epsilon$, $\{a_{n}\}$ converges to $L$

## If a sequence $\{a_{n}\}$ is decreasing and bounded below, then it converges to $\text{inf}(\{a_{n}:n\in\mathbb{N}\})$
Exactly same method, but using "$\text{inf}$" and "decreasing"

## Side Note
The statements "Every increasing bounded above sequence converges" and "Every decreasing bounded below sequence converges" are *equivalent to the Completeness Axiom*

# Subsequences
Informally, a subsequences is some **Infinite subset** of the original sequence, forming a new sequence
- Choose a sequence of natural numbers, $n_{1}<n_{2}<n_{3}\dots$, then the sequence is the terms $a_{n_{1}}, a_{n_{2}}\dots$
- Sequence itself is subsequence
- Since subsequence is skipping some indices, note that $n_{m}\geq m$

## Prop 28. If $\{a_{n}\}$ converges to $L$ and $\{a_{n_{m}}\}$ is some subsequence of $\{a_{n}\}$, then $\{a_{n_{m}}\}$ also converges to $L$
Let $\epsilon>0$. There is some $K$ so that $\forall \text{ }n>K$, $|a_{n}-L|<\epsilon$. Then for any $m>K$, since $n_{m}\geq m>K$, $|a_{n}-L|<\epsilon$ also. Thus, $\{a_{n_{m}}\}$ also converges to $L$

## How can we use this to prove that $\{1, -1, 1, -1\dots\}$ does not converge?
Let the odd term subsequence = $\{1,1,1,\dots\}$ and the even term subsequence = $\{-1, -1, \dots\}$ converges to different number. 

Prop 28 says that is a sequence converges, all subsequences must converge to the same value.
- Thus, it is not convergent

## Can a sequence have no convergent subsequence?
Yes
$\{a_{n}\}=\{n\}$, any subsequence of it is not bounded above, so since 
	(convergent)$\implies$ (bounded) by prop 24, 
no subsequence of it can converge

**Note)**
The sequence could be not bounded, but have a convergent subsequence
- $\{1,1,2,1,3,1,4,1,5,1\dots\}$ is not bounded but does have a convergent subsequence, $\{1,1,1,1\dots\}$

## For any sequence is bounded, does it always have at least one convergent subsequence?
Yes, this is true. This statement is called "Bolzano-Weierstraus Theorem"
1. Show that any sequence , bounded or not, has a monotone subsequence
2. Then use the monotone convergence theorem to prove this subsequence is convergent


