With Series, we want to make precise the notion of an "Infinite Sum"
- $\sum^{\infty}_{n=1}\frac{1}{n}$
- $0.9999\dots$

We want to think about these "Partial Sums" and what ehy converges to

# Partial Sums
Given any sequence $\{a_{n}\}$, its sequence of partial sums, written $\{A_{n}\}$ is the sequence defined by
$A_{1}=a_{1}$
$A_{2}=a_{1}+a_{2}$
$A_{3}=a_{1}+a_{2}+a_{3}$
 $\vdots$

**Q )**
For any $\{a_{n}\}$ is $\{A_{n}\}$ always increasing?
- No, Only if each $a_{n}\geq 0$

# Series
Given any sequence $\{a_{n}\}$ we say that 
$$\sum^{\infty}_{n=1}a_{n} $$
Converges to $L$, and write $$\sum^{\infty}_{n=1}a_{n}=L$$
If the sequence of partial sum $\{A_{n}\}$ converges to $L$.
- And call the expression $\sum^{n=1}_{\infty}a_{n}$ the Series associated to $a_{n}$

## Prop 34. If the series $\sum^{\infty}_{n=1}a_{n}$ converges to some $L$, then $\{a_{n}\}$ converges to 0
Suppose $\sum^{\infty}_{n=1}a_{n}$ converges to $L$
- I.e. the sequence of parital sums $\{A_{n}\}$ converges to $L$

Exercise) Show that the sequence $B_{n}=\{0, A_{1}, A_{2}, A_{3}\dots\}$ also converges to $L$

Then, 
$A_{1}-B_{1}=a_{1}$
$A_{2}-B_{2}=a_{2}$
$A_{3}-B_{3}=a_{3}$
 $\vdots$
i.e. $\forall \text{ }n\in\mathbb{N}, A_{n}-B_{n}=a_{n}$

Then, since $\{A_{n}\}$ and $\{B_{n}\}$ both converges to $L$, by the sequence arithmetic theorem, $\{a_{n}\}$ converges to 0

# Manipulating Infinite Series
We can manipuate
$$c\sum^{n}_{i=1}a_{i}=\sum^{n}_{i=1}ca_{i}  \text{ and }\sum^{n}_{i=1}(a_{i}+b_{i}) =\sum^{n}_{i=1}a_{n}+\sum^{n}_{i=1}b_{n}  $$

Note that we can rearrange the terms in finite sum and still get the same result. For infinite sum, it is possible to rearrange the terms and end up with a different sum

## Prop 35 Series Arithmetic Theorem
If $\sum^{\infty}_{n=1}a_{n}$ converges to $L$, then
1) $\forall \text{ } c\in\mathbb{R}, \text{ }$ $\sum^{\infty}_{n=1}ca_{n}$ converges to $cL$ **(Exercise)**
	- i.e. $\sum^{\infty}_{n=1}ca_{n}=c\cdot\sum^{\infty}_{n=1}a_{n}$

2) If $\sum^{\infty}_{n=1}b_{n}$ converges to $M$, then $\sum^{\infty}_{n=1}(a_{n}+b_{n})$ converges to $L+M$
	- i.e. $\sum^{\infty}_{n=1}(a_{n}+b_{n})=\sum^{\infty}_{n=1}a_{n}+\sum^{\infty}_{n=1}b_{n}$

## Example) Show $\sum^{\infty}_{n=1}\frac{1}{n}$ does not converge
We will show that sequence of partial sum is not Cauchy

Proof by Contradiction) Suppose it is Cauchy, do definition with $\epsilon=\frac{1}{2}$ will work
$$\exists \text{ }K\in\mathbb{R}\text{ such that }\forall \text{ }m,n>K, |A_{n}-A_{m}|<\frac{1}{2}$$

Suppose $m$ is some natural number $>K$, and let $n=2m$
Then, 
$$|A_{n}-A_{m}|=|A_{2m}-A_{m}|=\left|\sum^{2m}_{i=1}a_{i}-\sum^{m}_{i=1}a_{i}\right|$$
$$\left|\sum^{2m}_{i=m+1}a_{i}\right|=\frac{1}{m+1}+\frac{1}{m+2}+\frac{1}{m+3}\dots\frac{1}{2m}$$
$$\geq  \frac{1}{2m}+\frac{1}{2m}+\frac{1}{2m}\dots+\frac{1}{2m}=\frac{m}{2m}=\frac{1}{2}$$
$$\therefore|A_{n}-A_{m}|\geq  \frac{1}{2}$$

For any $K$, we have found $m,n>K$ so that $|A_{n}-A_{m}|\geq\frac{1}{2}$, so $\{A_{n}\}$ is not Cauchy

Since this contradicts the initial assumption, $\sum^{\infty}_{n=1}\frac{1}{n}$ does not converge

# Prop 36. Comparison Test
If $\{a_{n}\}$ and $\{b_{n}\}$ are sequences such that $\forall \text{ }n\in\mathbb{N}$, $0\leq a_{n}\leq b_{n}$. Then,
1) If $\sum^{\infty}_{n=1}b_{n}$ converges to $B$, $\sum^{\infty}_{n=1}a_{n}$ converges to some $A$ where $A\leq B$
2) If $\sum^{\infty}_{n=1}a_{n}$ does not converge, then $\sum^{\infty}_{n=1}b_{n}$ does not converge

**Prove 1)**
Since each $a_{n}\geq 0$, the sequence of partial sums $\{A_{n}\}$ is increasing.

Consider that $\{B_{n}\}$ also increasing and bounded above since it converges, by the Monotone Convergence Theorem, $\{B_{n}\}$ converges to $\text{sup}(\{B_{n}:n\in\mathbb{N}\})$, let it $B$

Then $\forall \text{ }n\in\mathbb{N}$, $A_{n}\leq B_{n}\leq B$, so $\{A_{n}\}$ is increasing and bounded above, then by Monotone Convergence Theorem, $\{A_{n}\}$ converges to $\text{sup}(\{A_{n}:n\in\mathbb{N}\})$, let it $A$

Since $B$ is an upper bound for $\{A_{n}\}$, $A\leq B$

**Prove 2)**
This is just a contrapositive of 1)

# Geometric Theorem
If $r\in\mathbb{R}$, then
1) If $|r|<1$, the series $\sum^{\infty}_{n=1}r^{n-1}$ converges to $\frac{1}{1-r}$
2) If $|r|\geq 1$, the series $\sum^{\infty}_{n=1}r^{n-1}$ does not converge
