# $\sigma$ Function
$\sigma$ is defined by setting $\sigma(n)$ equal to the sum of all positive divisor of $n$

**Ex)**
$\sigma(4) = 1+2+4=7$
$\sigma(9) = 1+3+9=13$

## Perfect Number
If $n\in\mathbb{Z}^{+}$ and $\sigma(n)=2n$ then $n$ is called a perfect number

## $\sigma(mn)$ is multiplicative
If $gcd(m,n)=1$, then $\sigma(mn)=\sigma(m)\sigma(n)$

Let $n=p^{a}$ where $p$ is prime, $a\in\mathbb{Z}^{+}$
- Then, $\sigma(n)=1+p+p^{2}\dots p^{a}$
- Since this is a geometric series, $\sigma(n)=\frac{p^{a+1}-1}{p-1}$

## Lemma 7.1 
For $n=p^{a}$ where $p$ is prime and $a\in\mathbb{Z}^{+}$, 
$$\sigma(n)=\frac{p^{a+1}-1}{p-1}$$


# Theorem 7.9
Let $n=p_{1}^{a_{1}}p_{2}^{a_{2}}\dots p_{k}^{a_{k}}$ be the prime power factorization of $n$, then
$$\sigma(n)=\prod^{k}_{i=1}\sigma(p_{i}^{a_{i}})$$
$$=\prod^{k}_{i=1}\left( \frac{p^{a_{i}+1}-1}{p_{i}-1} \right)$$

# Mersenne Prime
Consider Geometric Series
$$1+x+x^{2}+\dots x^{n-1}=\frac{x^{n}-1}{x-1}$$
$$(x-1)(1+x+x^{2}\dots x^{n-1})=x^{n}-1$$
So, $(x-1)\text{ | }(x^{n}-1)$

Assuming $x\in\mathbb{Z}, n\in \mathbb{Z}^{+}$, if $x>2$, then $x^{n}$ is composite
- Since $x-1$ which is neither $1$ nor $x^{n}-1$ can divide $x^{n}-1$

Then, consider when $x=2$
- Is $2^{n}-1$ prime or composite?
	- $n=2\implies 3$
	- $n= 4 \implies 15$
- It can be both

## $n$ is composite
Suppose $n$ is composite. Then $n=st$ for some $s,t\in\mathbb{Z}$, where $1<s\leq t<n$

Consider $2^{n}-1$
$$=(2^{s})^{t}-1$$
$$=(2^{s}-1)(1+2^{s}+(2^{s})^{2}\dots +(2^{s})^{t-2}+(2^{s})^{t-1})$$

Thus, 
$$(2^{s}-1)\text{ | }(2^{n}-1)$$
Since $s>1$, $2^{s}-1\neq 1$.
- Therefore, if $n$ is composite, then $2^{n}-1$ is also composite

## $n$ is prime
$2^{n}-1$ still can be prime or composite
- $2^{3}-1=7$
- $2^{11}-1 = 23\cdot 89$

## Mersenne Number / Mersenne Prime
Let $n\in\mathbb{Z}^{+}$. Then $M_{n}=2^{n}-1$  is the $n^{th}$ Mersenne number

Let $p$ is prime, if $M_{p} = 2^{p}-1$ is prime, then $M_{p}$ is a Mersenne Prime

## Theorem 7.10
Let $n$ be even positive integer. Then, $n$ is a perfect number iff $n=2^{m-1}(2^{m}-1)$ where $m\in\mathbb{Z}^{+},m\geq2$ and $2^{m}-1$ is prime

**Forward Direction)**
Suppose $n$ is even positive integer, $\sigma(n)2n$
Let $n=2^{s}t$ where $s,t\in\mathbb{Z}^{+}$ and $t$ is odd
$$\sigma(n)=2n=2^{s+1}t$$
Since $2$ and $t$ are relatively prime, 
$$\sigma(n)=\sigma(2^{s}t)=\sigma(2^{s})\sigma(t)=(2^{s+1}-1)\sigma(t)$$

Therefore, 
$$2^{s+1}t=(2^{s+1}-1)\sigma(t)$$
- Since $2^{s+1}$ is odd, $\sigma(t)$ must be even
- $\therefore{2}^{s+1}\text{ | }\sigma(t)$
- $\sigma(t)=2^{s+1}k$ $(k\in\mathbb{Z}^{+})$

So, 
$$2^{s+1}t=(2^{s+1}-1)2^{s+1}k$$
$$t=(2^{s+1}-1)k$$
- $k\neq t$ but $k\text{ | }t$
$$t=2^{s+1}k-k=\sigma(t)-k$$
1. If $k=1$, then $\sigma(t)=t+1\implies$ tells us that $t$ must be prime
2. If $k\neq 1$, then $t\neq 2^{s+1}-1$ and $(2^{s+1}-1)\text{ | }t$
	- Notes in Moodle


**Backward Direction)**
Suppose $2^{m}-1$ is prime for some $m\in\mathbb{Z}^{+}, m\geq 2$
- Then, $\sigma(2^{m}-1)=1+2^{m}-1=2^{m}$

Consider $\sigma(2^{m-1})$. Since this is sum of geometric series, 
- $=\frac{2^{m}-1}{2-1}=2^{m}-1$

Consider $\sigma(2^{m-1}(2^{m}-1))=\sigma(2^{m-1})\sigma(2^{m}-1)=2^{m}\cdot(2^{m}-1)=2(2^{m-1})(2^{m}-1)$
- Thus $2^{m-1}(2^{m}-1)$ is a perfect number
- Let's call this $n$
	- Then $n$ is even



