# Congruent
Let $a,b\in\mathbb{Z}$ and $m\in\mathbb{Z}^{+}$.
Then $a$ is congruent to "$b\text{ mod } m$" if $m\text{ | }(a-b)$
- $\exists \text{ }q\in\mathbb{Z}:mq=a-b\text{ / }a=mq+b$
- We write $a\equiv b(\text{mod }n)$

**Ex)**
$4\equiv 1(\text{mod 3})$
- $3\text{ | }(4-1)$

$1\equiv 4(\text{mod 3})$
- $3\text{ | }(1-4)$

$13\equiv -5(\text{mod 3})$
- $3\text{ | }(13-5)$

# Euclidean Algorithm
Computes GCD of 2 non-negative integers and is based on two things
1) If $r\in\mathbb{Z}^{+}$, then $gcd(r,0)=r$
2) Let $a,b$ integers and $b\neq 0$ and $q,r$ be integers such that $a=bq+r$. Then $gcd(a,b)=gcd(b,r)$

## Steps
1) Divide bigger number by smaller number
	- $a=bq+r$
2) Using Property (2), $gcd(a,b)=gcd(b,r)$
	- Note that $r$ is smaller number than $a,b$
3) Repeat this process until the pair is small enough to find GCD

**Ex)**
$gcd(18,12)$
- $18=12\cdot 1+6$
$=gcd(12,6)$
- $12=6\cdot 2+0$
$=gcd(6,0)$
$=6$

## Pseudocode
Input
- $a,b$ are non-negative integers, $a\geq b$

Initialization
- $A:=a, B:=b, R:=b$

Algorithmbody
- While $B \neq 0$:
	$R:= A\text{(mod B)}$
	$A:= B$
	$B:= R$

- $gcd:=A$

Output
- GCD

# Theorem 3.12
Let $f_{n+1}$and $f_{n+2}$ be any successive terms of the Fibonacci sequence with $n>1$, the Euclidean Algorithm takes $n$ divisions to show $gcd(f_{n+1}, f_{n+2})=1$



---
Let $a,b\in\mathbb{Z}$ such that $a>b>0$
Let $a=r_{0}, b=r_{1}$, then $a=bq_{1}+r_{2}$
- Then, $r_{0}=r_{1}q_{1}+r_{2}$ by substitution

Since $0<r_{2}<r_{1}$, $gcd(a,b)=gcd(r_{0}, r_{1})=gcd(r_{1},r_{2})$ 

Let $r_{1}=r_{2}q_{2}+r_{3}$
Then, since $0<r_{3}<r_{2}$, $gcd(a,b)=gcd(r_{0}, r_{1})=gcd(r_{1},r_{2})$ 
$\vdots$
$r_{n-2}=r_{n-1}q_{n-1}+r_{n}$
$r_{n-1}=r_{n}q_{n}+0$ $\leftarrow$ Terminates since remainder is 