# Proposition
If $ab\equiv x\text{ (mod }m)$ and $cd\equiv y\text{ (mod }m)$, then $abcd\equiv xy\text{ (mod }m)$

# Wilson's Theorem
If $p$ is prime, then $(p-1)!\equiv -1\text{ (mod }p)$

**Proof)**
Suppose $p$ is prime

i) If $p=2$, then $(p-1)\neq 1\equiv -1 \text{ (mod }2)$

ii) When $p>2$ ($p$ is odd)
Consider $a\in\{1,2,3\dots p-1\}$. Since $p$ is prime, $gcd(a,p)=1$

$\therefore$ a has inverse $\bar{a}$ modulo $p$

[[7. Conguents#Theorem 4.12|Theorem 4.12]]  told us $a^{2}\equiv 1 \text{ (mod }p)$ iff $a\equiv 1$ or $a\equiv -1 \text{ (mod }p)$
- So, the only integer in $\{1,2,\dots p-1\}$ that one their own inverses are 1 and $p-1$
- Thus, let's consier $\{2,3\dots p-1\}$

We group $2,3,\dots p-2$ into $\frac{p-3}{2}$ pairs that are congruent to $1\text{ (mod }p)$

**Claim)** No two integers in my list have the same inverse mod $p$

Proof by contradiction: Suppose $ax\equiv 1\text{ (mod }p)$ and $(a+j)x\equiv 1\text{ (mod }p)$
- $2\leq a,a+j, x\leq p-2$
- $1\leq j\leq p-3$
- $a,a+j\neq x$

Then,
- $p | ax-1$
- $p|(a+j)x-1$

$pq=ax-1$ for some $q\in \mathbb{Z}$
- Then $ax+jx-1=pq+jx \implies p|(pq+jx) \implies py=pq+jx$ for some $y\in\mathbb{Z}$
- $p(j-q)=jx$, thus $p|jx$. Since $p$ is prime, $p|j$ or $p|x$
- This contradicts that $x\leq p-2<p$ and $j\leq p-3<p$, thus $p$ can't divide $j$ and $x$
(End of proving Claim)

Then, by the clami, every integer in $\{2,3\dots p-2\}$ has distinct inverse mod $p$ from the set
- $2\cdot 3\dots(p-2)\equiv 1\text{ (mod }p)$

Therefore, $1\cdot 2\cdot 3\dots(p-1)\equiv p-1\equiv -1\text{ (mod }p)$