

---
# Theorem
Let $A$ be a matrix and $B$ for any matrix you can get to after finite number of element row operations from $A$. Then, $$\text{row}(A)=\text{row}(B)$$
**Proof)**
Rows of $B$ are linear combinations of rows of $A$
- $\forall \text{ }\vec{v}\in\text{row}(B)$, $\vec{v}\in\text{row}(A)$
- $\therefore\text{row}(B)\subseteq\text{row}(A)$

Similarly, we can express rows of $A$ in to linear combination of rows of $B$
- $\forall \text{ }\vec{u}\in\text{row}(A)$, $\vec{u}\in\text{row}(B)$
- $\therefore\text{row}(A)\subseteq\text{row}(B)$

Therefore, $\text{row}(A)=\text{row}(B)$

## Corollary: $\text{row}(A)=\text{row(R/REF(}A))$
Recall that $\text{rank}(A)=\text{\# non-zero rows in R/REF}(A)$
- These non-zero rows of $\text{R/REF}(A)$ form a basis for $\text{row}(A)$
- $\text{dim(row(R/REF}(A)))=\text{dim(row(}A))=\text{rank}(A)$

## $\text{rank}(A)=\text{dim(col(}A))$
$\text{rank}(A)=\text{\# non-zero rows in R/REF}(A)=\text{\# Leading elements in R/REF}(A)$
- But leading variable in a row in $\text{R/REF}$ is also a leading variable







- Essentially a column space basis = $\text{dim(col(}A))$

