# Separable Equations

Differential Equation that can be written as 
$$h(y)y' = g(x)$$
or
$$M(x)dx+N(y)dy=0$$
## Derive
$$M(x)dx+N(y)dy=0$$
$$\implies N(y)dy = -M(x)dx$$
$$\implies N(y) \frac{dy}{dx} = -M(x) \frac{dx}{dx}$$
$$\therefore N(y)y' = -M(x)$$
# Implicit Equation
Assume that $y$ is a solution

Let $G(x)$ and $H(y)$ be antiderivatives of $g(x)$ and $h(y)$

$$h(y)y' = g(x)$$
$$h(y)\cdot \frac{dy}{dx} = g(x)$$
$$h(y)dy = g(x)dx$$
$$\int h(y) \, dy  = \int g(x) \, dx $$
$$H(y) = G(x)+c$$
- Since this is not form of explicit solution( $y=f(x)+c$ ), this is an **implicit solution**
	- (Equation of $y$) = (Equation of $x$) + constant

# Constant Solution of Separable Equation
For DE
$$y' = g(x)p(y)$$
We need to divide $p(y)$, but this process is not valid if $p(y)=0$.
- We consider case $p(y)=0$ and $p(y)\neq 0$ separately

1. If $p(y)\neq 0$, then we will get implicit solution
2. If $p(y)=0$, regardless of $g(x)$, $y'=0$, thus $y$ is **constant solution**

# Definite Integral


## Example
$$y' = \frac{1}{2}x(1-y^2)$$
i) If $1-y^2\neq 0$
$$\frac{2y'}{y^{2}-1}= -x$$
$$[\frac{1}{{y-1}}-\frac{1}{y+1}]y' = -x$$
$$[\frac{1}{{y-1}}-\frac{1}{y+1}]\frac{dy}{dx} = -x$$
$$\int \frac{1}{{y-1}} \, dy -\int \frac{1}{{y+1}} \, dy  = \int -x \, dx $$
$$\ln|y-1|-\ln|y+1| = -\frac{1}{2}x^{2}+c$$
$$\ln|\frac{{y-1}}{{y+1}}| = -\frac{1}{2}x^2+c$$
- This is implicit solution

ii) If $1-y^{2}=0\longrightarrow y=\pm 1$, 
$$y' = \frac{1}{2}x(1-1) = 0$$
- $y=\pm 1$ are the constant solution



# Bernoulli Equation

$$y'+p(x)y = f(x)y^r$$
- Non-linear if $r\neq0,1$
	- Solve like [[1. Ordinary Differential Equation#Nonhomogeneous Equation|Non-homogenous Equation]]
		- Use Complementary Equation $y'+p(x)y=0$
	- Use $\frac{u'}{u^{r}} = f(x)\cdot(y_{1})^{r-1}$ instead of $u' = \frac{f(x)}{y_{1}}$

## Logic Behind
Similar to logic behind in [[1. Ordinary Differential Equation#Nonhomogeneous Equation#Logic behind|Non-homogenous Equation]]

Let $y_{1}$ is the solution of the complementary equation, then
$$y_{1}'+p(x)y_{1} = 0$$

From $y=uy_{1}$, 
$$y' = u'y_{1}+uy_{1}'$$
Therefore,
$$y'+p(x)y = f(x)y^r$$
$$\implies  u'y_{1}+uy_{1}'+p(x)(uy_{1}) = f(x)(uy_{1})^r$$
$$\implies u'y_{1}+u\{y_{1}'+p(x)y_{1}\} = f(x)(uy_{1})^r$$
Since $y_{1}'+p(x)y_{1} = 0$,  
$$\implies u'y_{1} = f(x)u^{r}y_{1}^r$$
$$\therefore \frac{u'}{u^{r}} = f(x)y_{1}^{r-1}$$

## Example
$$y'-y = xy^2$$
From complementary equation
$$y_{1}'-y_{1} = 0 \longrightarrow y_{1}=De^x$$
$$\frac{u'}{u^{r}} = f(x)\cdot(y_{1})^{r-1}$$
$$\implies \frac{u'}{u^{2}} = x\cdot(De^{x)^{2-1}}$$
$$\implies \frac{1}{u^{2}}du = (x\cdot De^{x})dx$$
$$\implies \int  \frac{1}{u^{2}}\, du  = \int  x\cdot De^{x}\, dx $$
$$\implies-\frac{1}{u} = D\cdot xe^x-De^x+c$$
$$\implies u=-\frac{1}{{De^{x}(x-1)+c}}$$

Using $y=uy_{1}$, 
$$y=uy_{1} = -\frac{1}{{De^{x}(x-1)+c}}\cdot De^x$$
Let constant $c = Dh$ with respect to another constant $h$
$$ -\frac{1}{{De^{x}(x-1)+Dh}}\cdot De^{x}= -\frac{1}{(x-1)+he^{-x}}$$
Therefore,
$$y=-\frac{1}{(x-1)+he^{-x}}$$






# Homogenous Nonlinear Equation
Nonlinear Equation that can be written as SE
- Focus on equations that can be written as ratio of $\frac{y}{x}$
$$y'=q(\frac{y}{x})$$
Let $u=\frac{y}{x}$, then $y=ux\implies y'=u'x+u$

## Steps
1. Find $u'$ from $y'=u'x+u$
2. Solve SE with respect to $u$
	- $y'=q(u)= u'x+u$
3. Find $y$ from $y=ux$

## Examples
Solve SE for
$$x^{2}y' = y^{2}+xy-x^{2}$$
Then, 
$$y'=\frac{y^{2}}{x^{2}}+\frac{xy}{x^{2}}-\frac{x^{2}}{x^{2}}$$
Let $u=\frac{y}{x}$, then
$$y' = u^{2}+u-1$$
Since $y=ux$, 
$$y'=u'x+u$$
$$\therefore u^{2}+u-1 = u'x+u \implies u'x=u^{2}-1$$
1) Constant Solution: What value of $u$ that makes $u'=0$
$$u=\pm 1 \implies u'x=0 \implies u'=0$$
$$u= \pm 1$$
are constant solution

2) Implicit solution
$$\frac{du}{dx} \frac{1}{u^{2}-1} = \frac{1}{x}$$
$$\frac{1}{u^{2}-1}du = \frac{1}{x}dx$$
$$\implies \frac{1}{2}\left( \frac{1}{u-1}-\frac{1}{u+1} \right) du = \frac{1}{x}dx$$
$$\implies \frac{1}{2}\left(\ln(u-1)-\ln(u+1) \right) = \ln x +c$$
$$\implies \ln\left( \frac{u-1}{u+1} \right) = 2\ln x+c$$
$$\implies \frac{u-1}{u+1} = e^{2\ln x+c} = Dx^{2}$$
$$\implies \frac{u-1}{u+1} = 1-\frac{2}{u+1} = Dx^{2}$$
$$\implies u=\frac{1+Dx^{2}}{1-Dx^{2}}$$

From 1), 
$$y=\pm x$$
From 2),
$$y=\left( \frac{1+Dx^{2}}{1-Dx^{2}} \right)\cdot x$$

$\to$ If $D \to 0 \implies u=1, y=x$
$\to$ If $D\to \infty \implies u=-1, y=-x$

