# CC Homogenous Equation
Homogenous equations that has
$$ay''+by'+cy=0$$
where $a(\neq 0),b,c$ are constant

## Characteristic Polynomial
The key of solving this DE is $y=e^{\lambda x}$, where $r$ is constant. Then 
$$ay''+by'+cy = a\lambda^{2}e^{\lambda x}+br e^{\lambda x}+ce^{\lambda x} = (a\lambda^{2}+b\lambda+c)e^{\lambda x}$$
The polynomial, $p(\lambda)=a\lambda^{2}+ b\lambda +c$ is called **characteristic polynomial**

Based on the quadratic formula and Discriminant $D$, from the characteristic polynomial, we can figure the number of roots and the value of $\lambda$

### If Discriminant $D>0$
Let $\lambda_{1}$ and $\lambda_{2}$ are the distinct real roots of characteristic polynomial, then according to [[7. Linear Second Order DE#General Solution| the general solution of SOLDE]], 
$$y=c_{1} e^{\lambda_{1} x}+c_{2} e^{\lambda_{2} x}$$
where $c_{1}$ and $c_{2}$ are just constant.

### If Discriminant $D=0$
If $D=0$, then the characteristic polynomial would have only one root, let it $\lambda_{0}$
- Since the original should not have another solution of form $e^{\lambda x}$, we are looking at $y=u\cdot y_{1} =u \cdot e^{\lambda x}$, where $u$ is *some function*

**Steps**
1. Substitute $y=u\cdot e^{\lambda x}$ to the original function and find the condition of $u$ that make the equation is satisfied
2. Express $u$ into two constants and $x$ so that it can be substitutable to $u\cdot e^{\lambda x}$
3. Use IC to calculate the value of constants

#### Example
Solve
$$y''+6y'+9y=0\text{ , }y(0)=3\text{ , }y'(0)=-1$$

From characteristic polynomial, 
$$\lambda^{2}+6\lambda+9=(\lambda+3)^{2}=0\implies\lambda=-3$$
Let $y=u\cdot e^{-3x}$, then
$$y'=u'e^{-3x}+ u\cdot(-3)e^{-3x}\text{ , }y''=u''e^{-3x}-6u'e^{-3x}+9u e^{-3x}$$$$\implies y''+6y'+9=e^{-3x}[u''-(6-6)u'+(9-18+9)u]=u''e^{-3x}$$
Then $y=u e^{-3x}$ would be solution to the original DE iff $u''=0$, thus $u=c_{1}+c_{2}x$
$$y=e^{-3x}(c_{1}+c_{2}x)$$
- $c_{1}=1, c_{2}=0$ yields $y_{1}=e^{-3x}$
- $c_{1}=0, c_{2}=1$ yields $y_{2}=xe^{-3x}$

Since $\frac{y_{2}}{y_{1}}$ is not constant, $y_{1}$ and $y_{2}$ are linearly independent, thus they form fundamental set

For IC,
substitute $y(0)=3$ and $y'(0)=-1$ and solve for $c_{1}$ and $c_{2}$
$\to$ $y=e^{-3x}(3+8x)$

### If Discriminant $D<0$
This condition will lead to complex root, let them $x+yi$ and $x-yi$. Then, rather than expressing $c_{1} \cdot e^{x+yi} +c_{2}\cdot e^{x-yi}$, we can express it as
$$y=c_{1} \cdot e^{(z+wi)x} +c_{2}\cdot e^{(z-wi)x} = c_{1}e^{wi\cdot x}\cdot e^{zx}+c_{2}e^{-wi\cdot x}\cdot e^{zx}$$
$$=(c_{1}e^{wi\cdot x}+c_{2}e^{-wi\cdot x})e^{zx}=u\cdot e^{zx}$$

**Steps**
1. Express $y'$ and $y''$ in terms of $x$ and $u$
2. Substitute 1. in the original function and simplify to form $f(x)\cdot g(u)$
3. Evaluate the condition of $u$ that makes RHS($f(x)\cdot g(u)$) equal to zero
4. Solve for $u$(constant appears here)
5. Use IC to calculate the constant

#### Example
Solve
$$y''+4y'+13y=0 \text{ , }y(0)=2 \text{ , } y'(0)=-3$$
Characteristic Polynomial:
$$p(\lambda)=\lambda^{2}+4\lambda+13 \implies \lambda = -2 \pm 3i$$
Then, 
$$y_{1} = e^{(-2+3i)x}, y_{2} = e^{(-2-3i)x} \implies y=u\cdot e^{-2x}$$
$$\implies y''+4y'+13y = e^{-2x}(u''+9u)$$

Thus, $y=ue^{-2x}$ is a solution for DE iff $u''+9u=0$

Then, $u=c_{1}\cos3x+c_{2}\sin 3x$ by granted theorem
$$\therefore y=e^{-2x}(c_{1} \cos 3x +c_{2} \sin 3x)$$


## General Solution
1. If characteristic polynomial has 2 unique real roots
$$y=c_{1}e^{\lambda_{1}x}+c_{2} e^{\lambda_{2} x}$$

2. If characteristic polynomial has 1 real root
$$y=e^{\lambda_{1} x}(c_{1}+c_{2} x)$$

3. If characteristic polynomial has 2 unique complex conjugate roots, $z \pm wi$
$$y=e^{z x}(c_{1} \cos (wx)+c_{2}\sin(wx))$$

# CC Non Homogenous DE
Homogenous equations that has
$$y''+p(x)y'+q(x)y=f(x)$$
where $f\neq 0$

## Uniqueness
Suppose $p, q, f$ are continuous on an open interval $(a,b)$, let $x_{0}$ be any point in $(a,b)$, and let $k_{0}$ and $k_{1}$ be arbitrary real number, then IVP
$$y''+p(x)y'+q(x)y=f(x) \text{ , } y(x_{0})=k_{0} \text{ , }y'(x_{0})=k_{1}$$
has a **unique solution** on $(a,b)$

## Particular Solution and General Solution
Let $y_{p}$ is a **particular solution** of 
$$y''+p(x)y'+q(x)y=f(x)$$
And for the complementary equation, 
$$y''+p(x)y'+q(x)y=0$$
let $\{y_{1}, y_{2}\}$ is fundamental set of this equation. 

Then the general solution of non-homogenous DE is
$$y=y_{p}+c_{1}y_{1}+c_{2}y_{2}$$

**Proof)**
- $y'=y_{p}'+c_{1}y_{1}'+c_{2}y_{2}'$ and $y''=y_{p}''+c_{1}y_{1}''+c_{2}y_{2}''$
- Substitute them in $y''+p(x)y'+q(x)y$ and simplify it to prove that it is equal to $f$

### Example
Solve
$$y''+y=1$$
$$y(0)=2 \text{ , } y'(0)=7$$
By inspection, $y_{p} = 1$
And since $y_{1} = \cos x$ and $y_{2} = \sin x$ form a fundamental set, 
$$y=1+c_{1}\cos x+c_{2}\sin x$$

By IC, 
$$y=1+\cos x+7\sin x$$


# Law of Superposition
If $y_{p_{1}}$ is particular solution of
$$y''+p(x)y'+q(x)y = f_{1}(x)$$
and $y_{p_{2}}$ is particular solution of 
$$y''+p(x)y'+q(x)y = f_{2}(x)$$
Then, $y_{p}=y_{p_{1}}+y_{p_{2}}$ is particular solution of 
$$y''+p(x)y'+q(x)y = f_{1}(x)+f_{2}(x)$$
- This can be easily extend and generalized that $y_{p}=y_{p_{1}}+y_{p_{2}}\dots y_{p_{i}}$ is particular solution of
$$y''+p(x)y'+q(x)y = f_{1}(x)+f_{2}(x)\dots f_{i}(x)$$

# Relation between behavior and $D$&Eigens
$D>0$ + positive two real $\lambda$ $\implies$ Exponential growth
$D>0$ + negative two real $\lambda$ $\implies$ Exponential decay
$D>0,b=0$ $\implies$ two real $\lambda$ $\implies$ Hyperbolic Solution
$D<0,b=0$ $\implies$ two imaginary $\lambda$ $\implies$ Oscillations
$D<0,b>0$ $\implies$ two imaginary $\lambda$ $\implies$ Decaying oscillations
$D<0,b<0$ $\implies$ two imaginary $\lambda$ $\implies$ Growth oscillations