# Exact Equation
Equation that has form of
$$M(x,y)dx+N(x,y)dy=0$$
or
$$M(x,y)+N(x,y)\frac{dy}{dx}=0$$
Then there is implicit solution $F(x,y)=c$ that
$$\frac{\partial }{\partial x}F(x,y) = M(x,y)\text{, }\frac{\partial }{\partial y}F(x,y) = N(x,y)$$

Since $M, N$ are partial derivative, 
$$M_{y}(x,y) = N_{x}(x,y)$$

## Example
Show that 
$$x^{4}y^{3}+x^{2}y^{5}+2xy=c$$
is an implicit solution of 
$$(4x^{3}y^{3}+2xy^{5}+2y)dx+(3x^{4}y^{2}+5x^{2}y^{4}+2x)dy=0$$
$\to$
$$\frac{\partial}{\partial x}\{x^{4}y^{3}+x^{2}y^{5}+2xy=c\}\to4x^{3}y^{3}+2xy^{5}+2y=0$$
$$\frac{\partial}{\partial y}\{x^{4}y^{3}+x^{2}y^{5}+2xy=c\}\to3x^{4}y^{2}+5x^{2}y^{4}+2x=0$$

# How to solve?
Step
1. Find $M(x,y)$ and $N(x,y)$
2. Integrate $M(x,y) \to F(x,y)=\int M(x,y) \, dx{}+\phi(y)$
3. Differentiate $F(x,y)$ we got from 2 with respect to $y$
4. Since $F_{y}(x,y) = N(x,y)$, find $\phi'(y)$
5. Integrate $\phi'(y)$ to get $\phi(y)$
6. Substitute $\phi(y)$ in $F(x,y)=\int M(x,y) \, dx+\phi(y)$ 

- This process can be done with $N(x,y)$ as well

